

Moment Generating Functions(mgf)

Definition:

Let X be a random variable. The moment generating function of X denoted by $M_X(t)$ and is defined as

$$M_X(t) = \begin{cases} \sum_{j=1}^{\infty} e^{tx_j} P(X=x_j); & X \text{ is discrete} \\ \int_{-\infty}^{\infty} e^{tx} f(x) dx; & X \text{ is continuous} \end{cases}$$

Note:

1. $M_X(t) = E(e^{tx})$
2. The nth derivative of $M_X(t)$ at $t = 0$ is $E(X^n)$. i.e., $M_X^{(n)}(0) = E(X^n)$.
3. $E(X^n)$ is the coefficient of $\frac{t^n}{n!}$ in the equation $M_X(t) = E(e^{tx})$.
4. $V(X) = M_X''(0) - [M_X'(0)]^2$.

Properties:

1. $M_{ax}(t) = M_X(at)$
2. $M_{ax+b}(t) = e^{tb} M_X(at)$
3. If X and Y are independent random variables, then $M_{X+Y}(t) = M_X(t) \cdot M_Y(t)$.
This can be generalized for 'n' random variables.
4. If two or more independent random variables having a certain distribution are added, the resulting random variable has a distribution of the same type as that of the random variables. This property is called reproductive property.
Example: Suppose that X and Y are independent random variables with distributions $N(\mu_1, \sigma_1^2)$ and $N(\mu_2, \sigma_2^2)$ respectively.

Let $Z = X + Y$.

$$M_X(t) = E(e^{zt}) = E(e^{(X+Y)t})$$

$$= E(e^{Xt}) \cdot E(e^{Yt}) = M_X(t) \cdot M_Y(t)$$

$$= e^{t\mu_1 + \frac{\sigma_1^2 t^2}{2}} \cdot e^{t\mu_2 + \frac{\sigma_2^2 t^2}{2}} = e^{t(\mu_1 + \mu_2) + (\sigma_1^2 + \sigma_2^2) \frac{t^2}{2}}$$

This represents the mgf of a normally distributed random variable with expected value $(\mu_1 + \mu_2)$ and variance $(\sigma_1^2 + \sigma_2^2)$.

Problems:

1. If X is the outcome obtained when a die is tossed, then find the moment generating function. Also find its mean and variance.

Solution: $P(X=x) = \frac{1}{6}; x=1,2,3,4,5,6$

We have $M_X(t) = E(e^{tx})$

$$= \sum_{x=1}^6 e^{tx} P(x)$$

$$= \frac{1}{6} [1 + e^t + e^{2t} + e^{3t} + e^{4t} + e^{5t} + e^{6t}]$$

We have $E(X) = M'_X(0) = \frac{1}{6} [1 + \dots + 6]$

$$= \frac{21}{6}$$

$$M''_X(t) = \frac{1}{6} [e^t + 4e^{2t} + \dots + 36e^{6t}]$$

$$E(X^2) = M''_X(0) = \frac{91}{6}$$

$$V(X) = M''_X(0) - [M'_X(0)]^2 = 2.91$$

2. If X is a random variable taking values 0,1,2,... and $P(X) = ab^x$, where a and b are positive constants such that $a+b = 1$, then

(i) Find mgf.

(ii) If $E(X) = m_1$, $E(X^2) = m_2$, show that $m_2 = m_1(2m_1 + 1)$.

Solution: (i): $M_X(t) = E(e^{tx})$

$$= \sum_{x=0}^{\infty} e^{tx} p(x) = \frac{a}{1 - be^t}$$

$$(ii): E(X) = M'_X(0) = \frac{ab}{(1-b)^2} = \frac{b}{a} = m_1$$

$$E(X^2) = m_2 = M''_X(0)$$

$$= \frac{b}{a} \left(\frac{1+b}{a} \right)$$

$$= m_1 \frac{1}{a} [a+b+b]$$

$$= m_1(2m_1 + 1)$$

3. If X has pdf $f(x) = \lambda e^{-\lambda(x-a)}$ if $x \geq a$. Find its mgf and also find the mean and variance.

4. Suppose that X has pdf $f(x) = \frac{e^{-|x|}}{2}$, $-\infty < x < \infty$, find mean and variance using mgf.

Mgf of Binomial distribution:

If $p(x) = nCx p^x q^{n-x}; x=0, 1, 2, \dots, n$, then

$$M_X(t) = \sum_{x=0}^n e^{tx} nCx p^x q^{n-x}$$

Expanding ,

$$M_X(t) = (pe^t + q)^n$$

Mgf of Poisson distribution:

If $p(x) = \frac{\alpha^x e^{-\alpha}}{x!}; x=0, 1, 2, \dots, \infty$, then

$$M_X(t) = \sum_{x=0}^{\infty} e^{tx} \frac{\alpha^x e^{-\alpha}}{x!}$$

$$= e^{-\alpha} e^{e^t \alpha}$$

$$= e^{\alpha(e^t - 1)}$$

Mgf of Uniform distribution in (-a, a):

If $f(x) = \frac{1}{2a}$ in $(-a, a)$, then

$$M_X(t) = \int_{-a}^a \frac{1}{2a} e^{tx} dx = \frac{\sinh at}{at}$$

The value of $E(X^{2n})$:

We know that $E(X^{2n})$ is the coefficient of $\frac{t^{2n}}{(2n)!}$ in the equation $M_X(t) = E(e^{tx})$.

$$E(X^{2n}) = \frac{a^{2n} t^{2n}}{(2n+1)!} = \frac{a^{2n}}{2n+1}$$

Mgf of Exponential distribution:

If $f(x) = \alpha e^{-\alpha x}, x > 0$, then

$$M_X(t) = \int_0^{\infty} \alpha e^{-\alpha x} e^{tx} dx$$

$$= \alpha \int_0^{\infty} e^{-(\alpha-t)x} dx$$

$$M_X(t) = \frac{\alpha}{\alpha - t}$$

Mgf of Gamma distribution:

If $f(x) = \frac{\alpha^r x^{r-1} e^{-\alpha x}}{\Gamma(r)}; \alpha > 0, r > 0, 0 < x < \infty$, then

$$M_X(t) = \int_0^{\infty} e^{tx} \frac{\alpha^r x^{r-1} e^{-\alpha x}}{\Gamma(r)} dx$$

$$\begin{aligned}
 \text{Take } x(\alpha - t) = v, \quad M_X(t) &= \frac{\alpha^r}{\Gamma(r)} \int_0^\infty \left(\frac{v}{\alpha - t} \right)^{r-1} e^{-v} \frac{dv}{\alpha - t} \\
 &= \frac{\alpha^r}{(\alpha - t)^r} \frac{1}{\Gamma(r)} \int_0^\infty e^{-v} v^{r-1} dv \\
 &= \frac{\alpha^r}{(\alpha - t)^r}
 \end{aligned}$$

Mgf of Chi-square distribution:

By substituting $r = \frac{n}{2}$, $\alpha = \frac{1}{2}$ in mgf of gamma distribution, we get chi-square distribution.

$$\text{Therefore } M_X(t) = (1 - 2t)^{-n/2}$$

Mgf of Normal distribution:

If $f(x) = \frac{1}{\sigma\sqrt{2\pi}} e^{-\frac{1}{2}\left(\frac{x-\mu}{\sigma}\right)^2}$, $-\infty < x < \infty$, then

$$M_X(t) = \frac{1}{\sigma\sqrt{2\pi}} \int_{-\infty}^{\infty} e^{tx} e^{-\frac{1}{2}\left(\frac{x-\mu}{\sigma}\right)^2} dx$$

$$\text{Substitute } z = \frac{x-\mu}{\sigma},$$

$$\begin{aligned}
 M_X(t) &= \frac{1}{\sigma\sqrt{2\pi}} \int_{-\infty}^{\infty} e^{t(\mu+\sigma z)} e^{-\frac{z^2}{2}} \sigma dz \\
 &= \frac{e^{t\mu}}{\sqrt{2\pi}} \int_{-\infty}^{\infty} e^{\frac{-1}{2}z^2} dz \\
 &= \frac{e^{t\mu} e^{\frac{\sigma^2 t^2}{2}}}{\sqrt{2\pi}} \int_{-\infty}^{\infty} e^{-\frac{1}{2}(z-t\sigma)^2} dz
 \end{aligned}$$

Substitute $y = z - t\sigma$ and use gamma function,

$$M_X(t) = e^{t\mu + \frac{\sigma^2 t^2}{2}}$$

Mgf of Standard normal distribution:

By substituting $\mu = 0$, $\sigma^2 = 1$, $\sigma = 1$ in mgf of normal distribution, we get the mgf of Standard normal distribution.

i.e.

$$M_X(t) = e^{t^2/2}$$